globals.v
@@ -15,76 +15,74 @@ Section Globals.
 
   Print sig.
 
-  Definition global_heap_lst (lst: varDefs) : Heap_type * Gamma_type * Env_type.
+  Definition global_heap_lst (lst: varDefs) : (* Heap_type * *)Gamma_type * Env_type.
     induction lst.
-    exact (p_heap.emptyPartFunc, p_gamma.emptyPartFunc, p_env.emptyPartFunc).
+    exact ((* p_heap.emptyPartFunc,  *)p_gamma.emptyPartFunc, p_env.emptyPartFunc).
     destruct IHlst.
-    destruct p.
+    (* destruct p. *)
     destruct a.
     rename c into C.
-    rename h into H.
+    (* rename h into H. *)
     rename e into L.
     rename p into Gamma.
-    set (o_fresh := ConcreteNamesAndTypes.vn.constructFresh (p_heap.domain H)).
-    destruct o_fresh as [o  o_fresh_proof].
+    (* set (o_fresh := ConcreteNamesAndTypes.vn.constructFresh (p_heap.domain H)). *)
+    (* destruct o_fresh as [o  o_fresh_proof]. *)
         
-    set (flds := fieldsList P C).
-    set (FM := p_FM.newPartFunc flds FM_null).
-    set (heapVal := obj C FM).
+    (* set (flds := fieldsList P C). *)
+    (* set (FM := p_FM.newPartFunc flds FM_null). *)
+    (* set (heapVal := obj C FM). *)
     split.
-    split.
-    exact (p_heap.updatePartFunc H o heapVal ).
+    (* split. *)
+    (* exact (p_heap.updatePartFunc H o heapVal ). *)
     exact (p_gamma.updatePartFunc Gamma v (typt_class C)).
-    exact (p_env.updatePartFunc L v (envRef o)).
+    exact (p_env.updatePartFunc L v envNull).
   Defined.
 
-  Definition globalEnv (P: Program) : Heap_type * Gamma_type * Env_type  :=
+  Definition globalEnv (P: Program) : (* Heap_type *  *)Gamma_type * Env_type  :=
     global_heap_lst (globals P).
 
-  Theorem WF_globals:
-    let (p, L) := globalEnv P in let (H, Gamma) := p in WF_Env P H Gamma L.
-    destruct P.
-    set (P' := {|
-     classDecls := classDecls;
-     globals := globals;
-     programBody := programBody;
-     programBodyIsTerm := programBodyIsTerm |}).
-    unfold globalEnv.
-    induction (syntax.globals P').
-    simpl.
-    split.
-    intro.
-    intro.
-    simpl in H.
-    elim H.
-    intros.
-    simpl in H.    
-    simplify_eq H.
+  (* Theorem WF_globals: *)
+  (*   let (p, L) := globalEnv P in let (H, Gamma) := p in WF_Env P H Gamma L. *)
+  (*   destruct P. *)
+  (*   set (P' := {| *)
+  (*    classDecls := classDecls; *)
+  (*    globals := globals; *)
+  (*    programBody := programBody; *)
+  (*    programBodyIsTerm := programBodyIsTerm |}). *)
+  (*   unfold globalEnv. *)
+  (*   induction (syntax.globals P'). *)
+  (*   simpl. *)
+  (*   split. *)
+  (*   intro. *)
+  (*   intro. *)
+  (*   simpl in H. *)
+  (*   elim H. *)
+  (*   intros. *)
+  (*   simpl in H.     *)
+  (*   simplify_eq H. *)
 
-    case_eq (global_heap_lst v).
-    intros.
-    destruct p.
-    rename H into hyp.
-    rename h into H; rename p into Gamma; rename e into L.
-    simpl.
-    rewrite hyp.
-    destruct a.
-    rename c into C.
-    rename v0 into x.
-    rename v into rest.
-    case_eq (ConcreteNamesAndTypes.vn.constructFresh (p_heap.domain H)).
-    intros o o_fresh.
-    intro dummy; clear dummy.
+  (*   case_eq (global_heap_lst v). *)
+  (*   intros. *)
+  (*   destruct p. *)
+  (*   rename H into hyp. *)
+  (*   rename h into H; rename p into Gamma; rename e into L. *)
+  (*   simpl. *)
+  (*   rewrite hyp. *)
+  (*   destruct a. *)
+  (*   rename c into C. *)
+  (*   rename v0 into x. *)
+  (*   rename v into rest. *)
+  (*   case_eq (ConcreteNamesAndTypes.vn.constructFresh (p_heap.domain H)). *)
+  (*   intros o o_fresh. *)
+  (*   intro dummy; clear dummy. *)
 
-    split.
-    rewrite hyp in IHv.
-    destruct IHv.
-    apply subset_preserved.
-    assumption.
+  (*   split. *)
+  (*   rewrite hyp in IHv. *)
+  (*   destruct IHv. *)
+  (*   apply subset_preserved. *)
+  (*   assumption. *)
 
-    (* Almost done!!! *)
-    admit.
-  Admitted.
+
     
     
 End Globals.
