heap.v
@@ -22,11 +22,11 @@ Section Heap.
 
   Definition heap_typeof (H: Heap_type) (o: Ref_type)
              (witn: In o (p_heap.domain H)) :
-    ClassName_type.
+    class.
     set (lem := proj2 (p_heap.fDomainCompat H o)).
     case_eq (p_heap.func H o).
     intros;    destruct b;    exact c.
-    intro is_none; set (is_absurd := lem is_none); auto.
+    intro is_none; set (is_absurd := lem is_none); firstorder.
   Defined.
 
 
