ocap.v
@@ -10,8 +10,8 @@ Section Ocap.
 
   Require Import Coq.Lists.List.
 
-  Print sig.
-
+    
+  (* Everything should be initialized to null... TODO: refactor*)
   Definition global_heap_lst (lst: varDefs) : Heap_type * Env_type.
     induction lst.
     exact (p_heap.emptyPartFunc, p_env.emptyPartFunc).
@@ -34,5 +34,85 @@ Section Ocap.
   Definition globalHeap (P: Program) : Heap_type * Env_type:=
     global_heap_lst (globals P).
 
+  Fixpoint noGlobals (env : list VarName_type) (t: ExprOrTerm) : Prop :=
+    match t with
+      | Null => True
+      | Var x => In x env
+      | FieldSelection x _ => In x env
+      | FieldAssignment x _ y => In x env /\ In y env
+      | MethodInvocation x _ z => In x env /\ In z env
+      | New _ => True
+      | Box _ => True
+
+      | Open x y t' => In x env /\ noGlobals (y :: env) t'
+      | TLet x e t' => noGlobals env e /\ noGlobals (x :: env) t'
+    end.
   
+  Definition methodNoGlobals (md: MethDecl) : Prop :=
+    noGlobals (var_name_this :: argName md :: nil) (methodBody md).
+
+  Definition classDeclNoGlobals (cd: ClassDecl) : Prop :=
+    Forall methodNoGlobals (methods cd).
+
+  Inductive directlyNotOcap (C: class) : Prop :=
+  | directlyNotOcapConstr :
+      forall cd,
+        lookup P C = Some cd ->
+        ~ classDeclNoGlobals cd ->
+        directlyNotOcap C.
+
+  Fixpoint directlyRelatedFieldlst (fs: flds) (A: class) :=
+    match fs with
+      | nil => False
+      | (_, A') :: fs' => A = A' \/ directlyRelatedFieldlst fs' A
+    end.
+
+  Definition directlyRelatedField (cd: ClassDecl) A := directlyRelatedFieldlst
+                                                         (cdFields cd) A.
+
   
+  Definition directlyRelatedTerm (t: ExprOrTerm) (A: class) :=
+    match t with
+      | New A' => A = A'
+      | _ => False
+    end.
+
+  Definition directlyRelatedMethod (md: MethDecl) A :=
+    argType md = typt_class A \/
+    directlyRelatedTerm (methodBody md) A.
+
+  
+  Inductive directlyRelated : class -> class -> Prop :=
+  | directlyRelatedByInheritance :
+      forall C_name B,
+        directlyRelated (extends C_name B) B
+
+  | directlyRelatedByMethod :
+      forall A cdA B,
+        lookup P A = Some cdA ->
+        Exists (fun md => directlyRelatedMethod md B)
+               (methods cdA) ->
+        directlyRelated A B
+
+  | directlyRelatedByField :
+      forall A cdA B,
+        directlyRelatedField cdA B ->
+        directlyRelated A B.
+
+  Require Import Coq.Relations.Relation_Operators.
+
+  Definition indirectlyRelated := clos_refl_trans_1n _ directlyRelated.
+
+  Inductive notOcap : class -> Prop :=
+  | notOcapConstr :
+      forall A B,
+        directlyNotOcap B ->
+        indirectlyRelated A B ->
+        notOcap A.
+
+  Definition ocap (C: class):  Prop :=
+    ~ notOcap C.
+    
+  
+End Ocap.
+
