makefile
@@ -1,17 +1,24 @@
-all: partial.vo namesAndTypes.vo syntax.vo classTable.vo heap.vo sframe.vo reductions.vo typing.vo wf_env.vo preservation.vo
+all: partial.vo namesAndTypes.vo syntax.vo classTable.vo heap.vo sframe.vo reductions.vo typing.vo wf_env.vo 
 
 %.vo : %.v
 	coqc $<
 
 
+
+## coqdep *v >> makefile
+
 classTable.vo classTable.glob classTable.v.beautified: classTable.v syntax.vo partial.vo namesAndTypes.vo
 classTable.vio: classTable.v syntax.vio partial.vio namesAndTypes.vio
 fs_preservation.vo fs_preservation.glob fs_preservation.v.beautified: fs_preservation.v syntax.vo partial.vo heap.vo classTable.vo sframe.vo reductions.vo typing.vo namesAndTypes.vo preservation.vo wf_env.vo
 fs_preservation.vio: fs_preservation.v syntax.vio partial.vio heap.vio classTable.vio sframe.vio reductions.vio typing.vio namesAndTypes.vio preservation.vio wf_env.vio
+globals.vo globals.glob globals.v.beautified: globals.v syntax.vo partial.vo namesAndTypes.vo heap.vo classTable.vo wf_env.vo
+globals.vio: globals.v syntax.vio partial.vio namesAndTypes.vio heap.vio classTable.vio wf_env.vio
 heap.vo heap.glob heap.v.beautified: heap.v syntax.vo namesAndTypes.vo classTable.vo
 heap.vio: heap.v syntax.vio namesAndTypes.vio classTable.vio
 namesAndTypes.vo namesAndTypes.glob namesAndTypes.v.beautified: namesAndTypes.v partial.vo
 namesAndTypes.vio: namesAndTypes.v partial.vio
+ocap.vo ocap.glob ocap.v.beautified: ocap.v syntax.vo partial.vo namesAndTypes.vo classTable.vo
+ocap.vio: ocap.v syntax.vio partial.vio namesAndTypes.vio classTable.vio
 partial.vo partial.glob partial.v.beautified: partial.v
 partial.vio: partial.v
 preservation.vo preservation.glob preservation.v.beautified: preservation.v syntax.vo partial.vo heap.vo classTable.vo sframe.vo reductions.vo typing.vo namesAndTypes.vo wf_env.vo
